Syscalls object added to distinguish from instructions

src/bin/init.cs
@@ -1,4 +1,4 @@
-// Dafny program test.dfy compiled into C#
+// Dafny program init.dfy compiled into C#
 // To recompile, you will need the libraries
 //     System.Runtime.Numerics.dll System.Collections.Immutable.dll
 // but the 'dotnet' tool in net5.0 should pick those up automatically.
@@ -8,15 +8,15 @@
 using System;
 using System.Numerics;
 [assembly: DafnyAssembly.DafnySourceAttribute(@"// Dafny 3.3.0.31104
-// Command Line Options: /home/alexis51151/Ecole/Rice University/COMP-517/comp517-project/src/dafny/test.dfy /verifyAllModules /spillTargetCode:1 /compile:3 /out:bin/test
-// test.dfy
+// Command Line Options: /home/alexis51151/Ecole/Rice University/COMP-517/comp517-project/src/dafny/init.dfy /verifyAllModules /spillTargetCode:1 /compile:3 /out:bin/init
+// init.dfy
 
-class Test {
-  method testProcess1()
+class Init {
+  method initProcess1()
   {
     var kernel: Kernel := new Kernel();
     var endokernel: Endokernel := new Endokernel(kernel);
-    var instruction: Instruction := Write('a', 0);
+    var instruction: Instruction := Instruction.Write('a', 0);
     var thread: Thread := new Thread(0, 0, 0, [instruction], endokernel);
     var p: Process := new Process(0, [0, 1, 2, 3], endokernel, thread);
     p.exec();
@@ -24,7 +24,7 @@ class Test {
 
   method Main()
   {
-    testProcess1();
+    initProcess1();
   }
 }
 
@@ -61,6 +61,7 @@ class Endokernel {
 
   method createEndoprocess(capability: Capability, instruction: Instruction) returns (endoprocess: Endoprocess)
     modifies this
+    ensures capability in capabilities && capabilities[capability] == endoprocess
     decreases capability, instruction
   {
     endoprocess := new Endoprocess(this.nextPid, capability.subspace, instruction, this);
@@ -90,8 +91,8 @@ class Endokernel {
     }
   }
 
-  method trapEndoprocess(instruction: Instruction, endoId: int)
-    decreases instruction, endoId
+  method trapEndoprocess(instruction: Instruction, syscall: Syscall, endoId: int)
+    decreases instruction, syscall, endoId
   {
     if instruction !in instructionMap {
       print ""trapEndoprocess error: no policy for this instruction\n"";
@@ -108,8 +109,10 @@ class Endokernel {
           if endoprocessTrapped != endoprocessExpected {
             print ""trapEndoprocess error: unknown endoprocess\n"";
           } else {
-            print ""Trapping back instruction from Endoprocess in Endokernel\n"";
-            kernel.exec(instruction);
+            print ""Trapping back syscall "";
+            print syscall;
+            print "" from Endoprocess in Endokernel\n"";
+            kernel.exec(syscall);
           }
         }
       }
@@ -123,7 +126,7 @@ class Endokernel {
     this.capabilities := map[];
     this.endoprocesses := map[];
     var capability: Capability := new Capability();
-    var instruction: Instruction := Write('a', 0);
+    var instruction: Instruction := Instruction.Write('a', 0);
     this.instructionMap := map[instruction := capability];
     this.kernel := kernel;
   }
@@ -133,6 +136,7 @@ class Endoprocess {
   var id: int
   var memorySpace: seq<int>
   var instructions: Instruction
+  var syscalls: map<Instruction, Syscall>
   var endokernel: Endokernel
 
   constructor (id: int, memorySpace: seq<int>, instructions: Instruction, endokernel: Endokernel)
@@ -142,21 +146,28 @@ class Endoprocess {
     this.memorySpace := memorySpace;
     this.instructions := instructions;
     this.endokernel := endokernel;
+    this.syscalls := map[Instruction.Write('a', 0) := Syscall.Write('a', 0), Instruction.Read(0) := Syscall.Read(0)];
   }
 
   method exec(instruction: Instruction)
     decreases instruction
   {
-    print ""Executing instruction in Endoprocess\n"";
-    endokernel.trapEndoprocess(instruction, this.id);
+    if instruction in syscalls {
+      print ""Executing syscall "";
+      print syscalls[instruction];
+      print "" in Endoprocess\n"";
+      endokernel.trapEndoprocess(instruction, syscalls[instruction], this.id);
+    }
   }
 }
 
 class Kernel {
-  method exec(instruction: Instruction)
-    decreases instruction
+  method exec(syscall: Syscall)
+    decreases syscall
   {
-    print ""Executing instruction in kernel\n"";
+    print ""Executing instruction "";
+    print syscall;
+    print "" in kernel\n"";
   }
 
   constructor ()
@@ -186,7 +197,9 @@ class Thread {
     modifies this, endokernel
   {
     if 0 <= pc < |instructions| {
-      print ""Executing instruction in Process\n"";
+      print ""Executing instruction "";
+      print instructions[pc];
+      print "" in Thread\n"";
       this.endokernel.trap(instructions[pc]);
       pc := pc + 1;
     }
@@ -209,6 +222,8 @@ class Capability {
     entries := [];
   }
 }
+
+datatype Syscall = Write(value: char, addr: int) | Read(addr: int)
 ")]
 
 //-----------------------------------------------------------------------------
@@ -1976,38 +1991,38 @@ namespace _System {
 } // end of namespace _System
 namespace _module {
 
-  public partial class Test {
-    public Test() {
+  public partial class Init {
+    public Init() {
     }
-    public void testProcess1()
+    public void initProcess1()
     {
-      Kernel _71_kernel;
+      Kernel _73_kernel;
       Kernel _nw0 = new Kernel();
       _nw0.__ctor();
-      _71_kernel = _nw0;
-      Endokernel _72_endokernel;
+      _73_kernel = _nw0;
+      Endokernel _74_endokernel;
       Endokernel _nw1 = new Endokernel();
-      _nw1.__ctor(_71_kernel);
-      _72_endokernel = _nw1;
-      Instruction _73_instruction;
-      _73_instruction = @Instruction.create_Write('a', BigInteger.Zero);
-      Thread _74_thread;
+      _nw1.__ctor(_73_kernel);
+      _74_endokernel = _nw1;
+      Instruction _75_instruction;
+      _75_instruction = @Instruction.create_Write('a', BigInteger.Zero);
+      Thread _76_thread;
       Thread _nw2 = new Thread();
-      _nw2.__ctor(BigInteger.Zero, BigInteger.Zero, BigInteger.Zero, Dafny.Sequence<Instruction>.FromElements(_73_instruction), _72_endokernel);
-      _74_thread = _nw2;
-      Process _75_p;
+      _nw2.__ctor(BigInteger.Zero, BigInteger.Zero, BigInteger.Zero, Dafny.Sequence<Instruction>.FromElements(_75_instruction), _74_endokernel);
+      _76_thread = _nw2;
+      Process _77_p;
       Process _nw3 = new Process();
-      _nw3.__ctor(BigInteger.Zero, Dafny.Sequence<BigInteger>.FromElements(BigInteger.Zero, BigInteger.One, new BigInteger(2), new BigInteger(3)), _72_endokernel, _74_thread);
-      _75_p = _nw3;
-      (_75_p).exec();
+      _nw3.__ctor(BigInteger.Zero, Dafny.Sequence<BigInteger>.FromElements(BigInteger.Zero, BigInteger.One, new BigInteger(2), new BigInteger(3)), _74_endokernel, _76_thread);
+      _77_p = _nw3;
+      (_77_p).exec();
     }
     public void _Main()
     {
-      (this).testProcess1();
+      (this).initProcess1();
     }
     public static void _StaticMain() {
-      Test _76_b = new Test();
-      _76_b._Main();
+      Init _78_b = new Init();
+      _78_b._Main();
     }
   }
 
@@ -2065,44 +2080,46 @@ namespace _module {
       if (!(this.instructionMap).Contains((instruction))) {
         Dafny.Helpers.Print(Dafny.Sequence<char>.FromString("trap error: no policy for this instruction\n"));
       } else {
-        Capability _77_capability;
-        _77_capability = Dafny.Map<Instruction, Capability>.Select(this.instructionMap,instruction);
-        Endoprocess _78_endoprocess = default(Endoprocess);
-        if (!(this.capabilities).Contains((_77_capability))) {
+        Capability _79_capability;
+        _79_capability = Dafny.Map<Instruction, Capability>.Select(this.instructionMap,instruction);
+        Endoprocess _80_endoprocess = default(Endoprocess);
+        if (!(this.capabilities).Contains((_79_capability))) {
           Endoprocess _out0;
-          _out0 = (this).createEndoprocess(_77_capability, instruction);
-          _78_endoprocess = _out0;
+          _out0 = (this).createEndoprocess(_79_capability, instruction);
+          _80_endoprocess = _out0;
         } else {
-          _78_endoprocess = Dafny.Map<Capability, Endoprocess>.Select(this.capabilities,_77_capability);
+          _80_endoprocess = Dafny.Map<Capability, Endoprocess>.Select(this.capabilities,_79_capability);
         }
         Dafny.Helpers.Print(Dafny.Sequence<char>.FromString("Trapping instruction "));
         Dafny.Helpers.Print(instruction);
         Dafny.Helpers.Print(Dafny.Sequence<char>.FromString(" from Process in Endokernel\n"));
-        (_78_endoprocess).exec(instruction);
+        (_80_endoprocess).exec(instruction);
       }
     }
-    public void trapEndoprocess(Instruction instruction, BigInteger endoId)
+    public void trapEndoprocess(Instruction instruction, Syscall syscall, BigInteger endoId)
     {
       if (!(this.instructionMap).Contains((instruction))) {
         Dafny.Helpers.Print(Dafny.Sequence<char>.FromString("trapEndoprocess error: no policy for this instruction\n"));
       } else {
-        Capability _79_capability;
-        _79_capability = Dafny.Map<Instruction, Capability>.Select(this.instructionMap,instruction);
-        if (!(this.capabilities).Contains((_79_capability))) {
+        Capability _81_capability;
+        _81_capability = Dafny.Map<Instruction, Capability>.Select(this.instructionMap,instruction);
+        if (!(this.capabilities).Contains((_81_capability))) {
           Dafny.Helpers.Print(Dafny.Sequence<char>.FromString("trapEndoprocess error: this endoprocess has not the required rights for such instruction\n"));
         } else {
-          Endoprocess _80_endoprocessExpected;
-          _80_endoprocessExpected = Dafny.Map<Capability, Endoprocess>.Select(this.capabilities,_79_capability);
+          Endoprocess _82_endoprocessExpected;
+          _82_endoprocessExpected = Dafny.Map<Capability, Endoprocess>.Select(this.capabilities,_81_capability);
           if (!(this.endoprocesses).Contains((endoId))) {
             Dafny.Helpers.Print(Dafny.Sequence<char>.FromString("trapEndoprocess error: unknown endoprocess\n"));
           } else {
-            Endoprocess _81_endoprocessTrapped;
-            _81_endoprocessTrapped = Dafny.Map<BigInteger, Endoprocess>.Select(this.endoprocesses,endoId);
-            if ((_81_endoprocessTrapped) != (object) (_80_endoprocessExpected)) {
+            Endoprocess _83_endoprocessTrapped;
+            _83_endoprocessTrapped = Dafny.Map<BigInteger, Endoprocess>.Select(this.endoprocesses,endoId);
+            if ((_83_endoprocessTrapped) != (object) (_82_endoprocessExpected)) {
               Dafny.Helpers.Print(Dafny.Sequence<char>.FromString("trapEndoprocess error: unknown endoprocess\n"));
             } else {
-              Dafny.Helpers.Print(Dafny.Sequence<char>.FromString("Trapping back instruction from Endoprocess in Endokernel\n"));
-              (this.kernel).exec(instruction);
+              Dafny.Helpers.Print(Dafny.Sequence<char>.FromString("Trapping back syscall "));
+              Dafny.Helpers.Print(syscall);
+              Dafny.Helpers.Print(Dafny.Sequence<char>.FromString(" from Endoprocess in Endokernel\n"));
+              (this.kernel).exec(syscall);
             }
           }
         }
@@ -2113,13 +2130,13 @@ namespace _module {
       (this).nextPid = BigInteger.Zero;
       (this).capabilities = Dafny.Map<Capability, Endoprocess>.FromElements();
       (this).endoprocesses = Dafny.Map<BigInteger, Endoprocess>.FromElements();
-      Capability _82_capability;
+      Capability _84_capability;
       Capability _nw5 = new Capability();
       _nw5.__ctor();
-      _82_capability = _nw5;
-      Instruction _83_instruction;
-      _83_instruction = @Instruction.create_Write('a', BigInteger.Zero);
-      (this).instructionMap = Dafny.Map<Instruction, Capability>.FromElements(new Dafny.Pair<Instruction, Capability>(_83_instruction, _82_capability));
+      _84_capability = _nw5;
+      Instruction _85_instruction;
+      _85_instruction = @Instruction.create_Write('a', BigInteger.Zero);
+      (this).instructionMap = Dafny.Map<Instruction, Capability>.FromElements(new Dafny.Pair<Instruction, Capability>(_85_instruction, _84_capability));
       (this).kernel = kernel;
     }
   }
@@ -2129,11 +2146,13 @@ namespace _module {
       this.id = BigInteger.Zero;
       this.memorySpace = Dafny.Sequence<BigInteger>.Empty;
       this.instructions = Instruction.Default();
+      this.syscalls = Dafny.Map<Instruction, Syscall>.Empty;
       this.endokernel = default(Endokernel);
     }
     public BigInteger id;
     public Dafny.ISequence<BigInteger> memorySpace;
     public Instruction instructions;
+    public Dafny.IMap<Instruction,Syscall> syscalls;
     public Endokernel endokernel;
     public void __ctor(BigInteger id, Dafny.ISequence<BigInteger> memorySpace, Instruction instructions, Endokernel endokernel)
     {
@@ -2141,20 +2160,27 @@ namespace _module {
       (this).memorySpace = memorySpace;
       (this).instructions = instructions;
       (this).endokernel = endokernel;
+      (this).syscalls = Dafny.Map<Instruction, Syscall>.FromElements(new Dafny.Pair<Instruction, Syscall>(@Instruction.create_Write('a', BigInteger.Zero), @Syscall.create_Write('a', BigInteger.Zero)), new Dafny.Pair<Instruction, Syscall>(@Instruction.create_Read(BigInteger.Zero), @Syscall.create_Read(BigInteger.Zero)));
     }
     public void exec(Instruction instruction)
     {
-      Dafny.Helpers.Print(Dafny.Sequence<char>.FromString("Executing instruction in Endoprocess\n"));
-      (this.endokernel).trapEndoprocess(instruction, this.id);
+      if ((this.syscalls).Contains((instruction))) {
+        Dafny.Helpers.Print(Dafny.Sequence<char>.FromString("Executing syscall "));
+        Dafny.Helpers.Print(Dafny.Map<Instruction, Syscall>.Select(this.syscalls,instruction));
+        Dafny.Helpers.Print(Dafny.Sequence<char>.FromString(" in Endoprocess\n"));
+        (this.endokernel).trapEndoprocess(instruction, Dafny.Map<Instruction, Syscall>.Select(this.syscalls,instruction), this.id);
+      }
     }
   }
 
   public partial class Kernel {
     public Kernel() {
     }
-    public void exec(Instruction instruction)
+    public void exec(Syscall syscall)
     {
-      Dafny.Helpers.Print(Dafny.Sequence<char>.FromString("Executing instruction in kernel\n"));
+      Dafny.Helpers.Print(Dafny.Sequence<char>.FromString("Executing instruction "));
+      Dafny.Helpers.Print(syscall);
+      Dafny.Helpers.Print(Dafny.Sequence<char>.FromString(" in kernel\n"));
     }
     public void __ctor()
     {
@@ -2185,7 +2211,9 @@ namespace _module {
     public void exec()
     {
       if (((this.pc).Sign != -1) && ((this.pc) < (new BigInteger((this.instructions).Count)))) {
-        Dafny.Helpers.Print(Dafny.Sequence<char>.FromString("Executing instruction in Process\n"));
+        Dafny.Helpers.Print(Dafny.Sequence<char>.FromString("Executing instruction "));
+        Dafny.Helpers.Print((this.instructions).Select(this.pc));
+        Dafny.Helpers.Print(Dafny.Sequence<char>.FromString(" in Thread\n"));
         (this.endokernel).trap((this.instructions).Select(this.pc));
         (this).pc = (this.pc) + (BigInteger.One);
       }
@@ -2295,9 +2323,93 @@ namespace _module {
       (this).entries = Dafny.Sequence<Dafny.ISequence<char>>.FromElements();
     }
   }
+
+  public abstract class Syscall {
+    public Syscall() { }
+    private static readonly Syscall theDefault = create_Write('D', BigInteger.Zero);
+    public static Syscall Default() {
+      return theDefault;
+    }
+    private static readonly Dafny.TypeDescriptor<Syscall> _TYPE = new Dafny.TypeDescriptor<Syscall>(Syscall.Default());
+    public static Dafny.TypeDescriptor<Syscall> _TypeDescriptor() {
+      return _TYPE;
+    }
+    public static Syscall create_Write(char @value, BigInteger addr) {
+      return new Syscall_Write(@value, addr);
+    }
+    public static Syscall create_Read(BigInteger addr) {
+      return new Syscall_Read(addr);
+    }
+    public bool is_Write { get { return this is Syscall_Write; } }
+    public bool is_Read { get { return this is Syscall_Read; } }
+    public char dtor_value {
+      get {
+        var d = this;
+        return ((Syscall_Write)d).@value; 
+      }
+    }
+    public BigInteger dtor_addr {
+      get {
+        var d = this;
+        if (d is Syscall_Write) { return ((Syscall_Write)d).addr; }
+        return ((Syscall_Read)d).addr; 
+      }
+    }
+  }
+  public class Syscall_Write : Syscall {
+    public readonly char @value;
+    public readonly BigInteger addr;
+    public Syscall_Write(char @value, BigInteger addr) {
+      this.@value = @value;
+      this.addr = addr;
+    }
+    public override bool Equals(object other) {
+      var oth = other as Syscall_Write;
+      return oth != null && this.@value == oth.@value && this.addr == oth.addr;
+    }
+    public override int GetHashCode() {
+      ulong hash = 5381;
+      hash = ((hash << 5) + hash) + 0;
+      hash = ((hash << 5) + hash) + ((ulong)Dafny.Helpers.GetHashCode(this.@value));
+      hash = ((hash << 5) + hash) + ((ulong)Dafny.Helpers.GetHashCode(this.addr));
+      return (int) hash;
+    }
+    public override string ToString() {
+      string s = "Syscall.Write";
+      s += "(";
+      s += Dafny.Helpers.ToString(this.@value);
+      s += ", ";
+      s += Dafny.Helpers.ToString(this.addr);
+      s += ")";
+      return s;
+    }
+  }
+  public class Syscall_Read : Syscall {
+    public readonly BigInteger addr;
+    public Syscall_Read(BigInteger addr) {
+      this.addr = addr;
+    }
+    public override bool Equals(object other) {
+      var oth = other as Syscall_Read;
+      return oth != null && this.addr == oth.addr;
+    }
+    public override int GetHashCode() {
+      ulong hash = 5381;
+      hash = ((hash << 5) + hash) + 1;
+      hash = ((hash << 5) + hash) + ((ulong)Dafny.Helpers.GetHashCode(this.addr));
+      return (int) hash;
+    }
+    public override string ToString() {
+      string s = "Syscall.Read";
+      s += "(";
+      s += Dafny.Helpers.ToString(this.addr);
+      s += ")";
+      return s;
+    }
+  }
 } // end of namespace _module
 class __CallToMain {
   public static void Main(string[] args) {
-    Dafny.Helpers.WithHaltHandling(_module.Test._StaticMain);
+    Dafny.Helpers.WithHaltHandling(_module.Init._StaticMain);
   }
 }
