src/dafny/Endo.dfy
@@ -1,6 +1,7 @@
 include "Capability.dfy"
 include "Kernel.dfy"
 include "Instructions.dfy"
+include "Syscalls.dfy"
 
 class Endokernel {
     var capabilities: map<Capability, Endoprocess>
@@ -9,14 +10,17 @@ class Endokernel {
     var nextPid:int;
     var kernel:Kernel;
 
-    method createEndoprocess(capability:Capability, instruction:Instruction) returns (endoprocess:Endoprocess) modifies this {
+    method createEndoprocess(capability:Capability, instruction:Instruction) returns (endoprocess:Endoprocess) modifies this 
+        ensures capability in capabilities && capabilities[capability] == endoprocess;
+    {
         endoprocess := new Endoprocess(this.nextPid, capability.subspace, instruction, this);
         this.capabilities := capabilities[capability := endoprocess];
         this.endoprocesses := this.endoprocesses[this.nextPid := endoprocess];
         this.nextPid := nextPid + 1;
     }
 
-    method trap(instruction:Instruction) modifies this  { 
+    method trap(instruction:Instruction) modifies this    
+      { 
         if (instruction !in instructionMap){
            print "trap error: no policy for this instruction\n";
         } 
@@ -29,14 +33,14 @@ class Endokernel {
                 endoprocess := capabilities[capability];
             }
             
-            print "Trapping instruction";
+            print "Trapping instruction ";
             print instruction;
-            print "from Process in Endokernel\n";
+            print " from Process in Endokernel\n";
             endoprocess.exec(instruction);
         }
     }
 
-    method trapEndoprocess(instruction:Instruction, endoId:int) {
+    method trapEndoprocess(instruction:Instruction, syscall:Syscall, endoId:int) {
         // Verifying if endoprocess has correct access rights to execute this instruction
         if (instruction !in instructionMap){
            print "trapEndoprocess error: no policy for this instruction\n";
@@ -56,8 +60,10 @@ class Endokernel {
                         print "trapEndoprocess error: unknown endoprocess\n";
                     }
                     else {
-                        print "Trapping back instruction from Endoprocess in Endokernel\n";
-                        kernel.exec(instruction);
+                        print "Trapping back syscall ";
+                        print syscall;
+                        print " from Endoprocess in Endokernel\n";
+                        kernel.exec(syscall);
                     }
                 }
             }
@@ -70,7 +76,7 @@ class Endokernel {
         this.capabilities := map[];
         this.endoprocesses := map[];
         var capability:Capability := new Capability();
-        var instruction:Instruction := Write('a', 0);
+        var instruction:Instruction := Instruction.Write('a', 0);
         this.instructionMap := map[instruction := capability];
         this.kernel := kernel;
     }
@@ -80,6 +86,7 @@ class Endoprocess {
     var id:int;
     var memorySpace:seq<int>
     var instructions: Instruction
+    var syscalls:map<Instruction, Syscall>
     var endokernel:Endokernel;
 
     constructor(id:int, memorySpace:seq<int>, instructions:Instruction, endokernel:Endokernel) {
@@ -87,10 +94,17 @@ class Endoprocess {
         this.memorySpace := memorySpace;
         this.instructions := instructions;
         this.endokernel := endokernel;
+        // Definition of the allowed syscalls and mapping between instructions and syscalls
+        this.syscalls := map[Instruction.Write('a', 0) := Syscall.Write('a',0),
+                             Instruction.Read(0) := Syscall.Read(0)];
     }
 
     method exec(instruction:Instruction)  {
-        print "Executing instruction in Endoprocess\n";
-        endokernel.trapEndoprocess(instruction, this.id);
+        if (instruction in syscalls) {
+            print "Executing syscall ";
+            print syscalls[instruction];
+            print " in Endoprocess\n";
+            endokernel.trapEndoprocess(instruction, syscalls[instruction], this.id);
+        }
     }
 }
