src/dafny/Syscalls.dfy
@@ -1,0 +1,3 @@
+datatype Syscall = 
+    Write(value:char, addr:int) 
+    | Read(addr:int)
